Tools.fst
@@ -1,0 +1,7 @@
+module Tools
+
+let (@@) #a #b #c (f: b -> c) (g: a -> b) (v:a) = f (g v) 
+
+let ( |> ) (v:'a) (f: 'a -> 'b): 'b = f v
+let ( <| ) (f: 'a -> 'b) (v:'a): 'b = f v
+
