prog-example/fib.c.pp
@@ -1,6 +1,9 @@
-
+function heeee (a) {
+d = 3
+}
 asdsad = 23; 
 current = 1; 
+SKIP; 
 previous = 1; 
 i = 0; 
 hey = 2; 
@@ -16,4 +19,8 @@ while (i <= 16) {
     hey = hey + 24
 }; 
 x = 100; 
-x = x / 7
+x = x / 3; 
+blou = 3; 
+while (blou <= 40) {
+    blou = blou + 5
+}
